Improvements in traits test case

Test/dafny0/Trait/TraitExample.dfy
@@ -4,79 +4,148 @@
 trait Automobile {
   ghost var Repr: set<object>
   predicate Valid()
-    reads this //, Repr
+    reads this, Repr
     ensures Valid() ==> this in Repr
   function method Brand(): string
   var position: int
   method Drive()
     requires Valid()
-    modifies this // Repr
+    modifies Repr
+    ensures Valid() && fresh(Repr - old(Repr))
     ensures old(position) <= position
-}
-
-class Volvo extends Automobile {
-  predicate Valid()
-    reads this //, Repr
-    ensures Valid() ==> this in Repr
-  {
-    this in Repr
-  }
-  constructor()
-    modifies this
-    ensures Valid()
-  {
-    Repr := {this};
-  }
-  function method Brand(): string {
-    "Volvo"
-  }
-  method Drive()
-//    requires Valid()
-    modifies this // Repr
-    ensures old(position) <= position
-  {
-    position := position + 10;
-  }
 }
 
 class Fiat extends Automobile {
   predicate Valid()
-    reads this // , Repr
+    reads this, Repr
     ensures Valid() ==> this in Repr
   {
-    this in Repr
+    this in Repr && null !in Repr && position <= 100
   }
-  constructor()
+  constructor (pos: int)
+    requires pos <= 100
     modifies this
-    ensures Valid()
+    ensures Valid() && fresh(Repr - {this}) && position == pos
   {
-    Repr := {this};
+    position, Repr := pos, {this};
   }
   function method Brand(): string {
     "Fiat"
   }
   method Drive()
-//    requires Valid()
-    modifies this // Repr
+    requires Valid()
+    modifies Repr
+    ensures Valid() && fresh(Repr - old(Repr))
     ensures old(position) <= position
   {
-    position := position + 3;
+    position := if position < 97 then position + 3 else 100;
+  }
+}
+
+class Volvo extends Automobile {
+  var odometer: Odometer
+  predicate Valid()
+    reads this, Repr
+    ensures Valid() ==> this in Repr
+  {
+    this in Repr && null !in Repr && odometer in Repr &&
+    position % 10 == 0 &&  // position is always a multiple of 10
+    odometer.value == position
+  }
+  constructor ()
+    modifies this
+    ensures Valid() && fresh(Repr - {this})
+  {
+    position, Repr := 0, {this};
+    odometer := new Odometer();
+    Repr := Repr + {odometer};
+  }
+  function method Brand(): string {
+    "Volvo"
+  }
+  method Drive()
+    requires Valid()
+    modifies Repr
+    ensures Valid() && fresh(Repr - old(Repr))
+    ensures old(position) < position  // always promises to make a move
+  {
+    position := position + 10;
+    odometer.Advance(10);
+  }
+}
+
+class Odometer {
+  var value: int
+  constructor ()
+    modifies this
+    ensures value == 0
+  {
+    value := 0;
+  }
+  method Advance(d: int)
+    requires 0 <= d
+    modifies this
+    ensures value == old(value) + d
+  {
+    value := value + d;
+  }
+}
+
+class Catacar extends Automobile {
+  var f: Fiat
+  var v: Volvo
+  predicate Valid()
+    reads this, Repr
+    ensures Valid() ==> this in Repr
+  {
+    this in Repr && null !in Repr &&
+    f in Repr && this !in f.Repr && f.Repr <= Repr && f.Valid() &&
+    v in Repr && this !in v.Repr && v.Repr <= Repr && v.Valid() &&
+    f.Repr !! v.Repr &&
+    position == f.position + v.position
+  }
+  constructor ()
+    modifies this
+    ensures Valid() && fresh(Repr - {this})
+  {
+    Repr := {this};
+    f := new Fiat(0);  Repr := Repr + f.Repr;
+    v := new Volvo();  Repr := Repr + v.Repr;
+    position := v.position;
+  }
+  function method Brand(): string {
+    "Catacar"
+  }
+  method Drive()
+    requires Valid()
+    modifies Repr
+    ensures Valid() && fresh(Repr - old(Repr))
+    ensures old(position) <= position
+  {
+    f := new Fiat(f.position);
+    f.Drive();  v.Drive();
+    Repr := Repr + v.Repr + f.Repr;
+    position := f.position + v.position;
   }
 }
 
 method Main() {
   var auto: Automobile;
+  auto := new Fiat(0);
+  WorkIt(auto);
   auto := new Volvo();
   WorkIt(auto);
-  auto := new Fiat();
+  auto := new Catacar();
   WorkIt(auto);
 }
 
 method WorkIt(auto: Automobile)
   requires auto != null && auto.Valid()
-  modifies auto // auto.Repr
+  modifies auto.Repr
 {
   auto.Drive();
+  auto.Drive();
+  assert old(auto.position) <= auto.position;
   print auto.Brand(), ": ", auto.position, "\n";
-  auto.position := 0;
+  auto.position := 18;  // note, this may destroy the automobile's consistency condition (given by Valid)
 }
